

Practical - 6

Aim :- Differential Equations

a) Solve differential equation.

`x = var('x')`

`y = function('y')(x)`

`de = diff(y, x) == (x * (1 - x^2)) / (y * (2 - y))`

`sol = desolve(de, y)`

`show(sol)`

OUTPUT :-

$$\frac{1}{3} y(x)^3 - y(x)^2 = \frac{1}{4} x^4 - \frac{1}{2} x^2 + C$$

b) Solve differential equation using initial value problem.

`x = var('x')`

`y = function('y')(x)`

`de = diff(y, x) == (x * (1 - x^2)) / (y * (2 - y))`

`sol = desolve(de, y)`

`show(sol)`

`sol2 = desolve(de, y, ics = [0, 1])`

`show(sol2)`

OUTPUT :-

$$\frac{1}{3} y(x)^3 - y(x)^2 = \frac{1}{4} x^4 - \frac{1}{2} x^2 + C$$

$$\frac{1}{3} y(x)^3 - y(x)^2 = \frac{1}{4} x^4 - \frac{1}{2} x^2 - \frac{2}{3}$$

c) Numerical solution of first-order equations using Euler's method.

Code:

```
def euler(f, x0, y0, h, x1):  
    n = int((1.0) * (x1 - x0) / h)  
    xv, yv = x0, y0  
    soln = [[x0, y0]]  
    for i in range(1, n+1):  
        xv = x0 + (h * i)  
        yv = yv + (h * f(xv, yv))  
        soln.append([xv, yv])  
    return soln
```

var('x, y')

$f(x, y) = (x * (1 - x^2)) / (y * (y - 2))$

x0 = 0

y0 = 1

h = 0.1

x1 = 1

euler(f, x0, y0, h, x1)

OUTPUT:-

[0, 1]

[0.10000000000000000, 0.99010000000000000]

[0.20000000000000000, 0.970898118023547]

[0.30000000000000000, 0.943574977522111]

[0.40000000000000000, 0.909867660734499]

[0.50000000000000000, 0.872060521639262]

[0.60000000000000000, 0.833021511201714]

[0.70000000000000000, 0.796297581357226]

[0.80000000000000000, 0.766250799915668]

$$1) \frac{dy}{dx} = \frac{x(1-x^2)}{y(2-y)}$$

$$y(2-y)dy = x(1-x^2)dx$$

$$y(y-2)dy = x(x^2-1)dx$$

$$(y^2 - 2y)dy = (x^3 - x)dx$$

Integrate on b.t.s.,

$$\int (y^2 - 2y)dy = \int (x^3 - x)dx$$

$$\int y^2 dy - \int 2y dy = \int x^3 dx - \int x dx$$

$$\frac{y^3}{3} - 2 \int \frac{y^2}{2} = \frac{x^4}{4} - \frac{x^2}{2} + C$$

$$\frac{y^3}{3} - y^2 = \frac{x^4}{4} - \frac{x^2}{2} + C$$

$$2) (x, y) = (0, 1)$$

$$\therefore \frac{y^3}{3} - y^2 = \frac{x^4}{4} - \frac{x^2}{2} + C$$

$$\therefore \frac{(1)^3}{3} - (1)^2 = \frac{(10)^4}{4} - \frac{(10)^2}{2} + C$$

$$\frac{1}{3} - 1 = C$$

$$C = \frac{1-3}{3}$$

$$C = \frac{-2}{3}$$

$$\therefore \frac{y^3}{3} - y^2 = \frac{x^4}{4} - \frac{x^2}{2} - \frac{2}{3}$$

3) $f(x, y) = \frac{x(1-x^2)}{y(y-2)}$; $x_0 = 0, y_0 = 1, \Delta x = 0.1$

i	x_i	y_i
0	0	1
1	0.1	0.9901
2	0.2	0.9709
3	0.3	0.9438

Put, $x = 0$

$$y_{0+1} = y_0 + f(x_0, y_0) \Delta x$$

$$y_1 = 1 + f(x_0, y_0) (0.1)$$

$$\therefore f(x_0, y_0) = \frac{x_0(1-x_0^2)}{y_0(y_0-2)} \quad \therefore f(x_0, y_0) = \frac{x_0(1-x_0^2)}{y_0(y_0-2)}$$

$$\therefore y_1 = 1 + (0)(0.1)$$

$$= 1$$

$$= \frac{0(1-0^2)}{1(1-2)}$$

$$=$$

Put, $x = 1$

$$y_{1+1} = y_1 + f(x_1, y_1) \Delta x$$

$$y_2 = 1 + f(x_1, y_1) (0.1)$$

$$\therefore f(x_1, y_1) = \frac{x_1(1-x_1^2)}{y_1(y_1-2)}$$

$$=$$

$$= \frac{(0.1)(1 - (0.1)^2)}{1(1 - 2)}$$

$$= \frac{(0.1)(1 - 0.01)}{-1}$$

$$= - (0.1)(0.99)$$

$$= -0.099$$

$$\therefore y_2 = 1 - 0.099(0.1)$$

$$= 1 - 0.0099$$

$$= 0.9901$$

$$\text{Put } x = 2$$

$$y_{2+1} = y_2 + f(x_2, y_2) \Delta x$$

$$y_3 = 0.9901 + f(x_2, y_2)(0.1)$$

$$\therefore f(x_2, y_2) = \frac{x_2(1 - x_2^2)}{y_2(y_2 - 2)} = \frac{(0.2)(1 - (0.2)^2)}{(0.99)(0.99 - 2)}$$

$$= \frac{-0.192}{0.9999} \approx -0.192$$

$$y_3 = 0.9901 - 0.192(0.1)$$

$$= 0.9901 - 0.0192$$

$$= 0.9709$$

$$\text{Put } x = 3$$

$$y_{3+1} = y_3 + f(x_3, y_3) \Delta x$$

$$y_4 = 0.9709 + f(x_3, y_3)(0.1)$$

$$\therefore f(x_3, y_3) = \frac{x_3(1 - x_3^2)}{y_3(y_3 - 2)}$$

$$= \frac{0.3(1 - (0.3)^2)}{0.9709(0.9709 - 2)}$$

$$= \frac{0.231}{-1.0291} \approx -0.224$$

$$= \frac{-0.273}{0.999}$$

$$0.999$$

$$\approx -0.2732$$

$$\therefore Y_4 = 0.9709 - 0.2732(0.1)$$

$$= 0.9709 - 0.02732$$

$$= 0.94358$$

Practical - 7

Aim :- First order partial order

```
1) var('x, y')  
f(x, y) = (x*y) / (x + y)  
fx = f.diff(x)  
show(fx(x, y))  
fy = f.diff(y)  
show(fy(x, y))
```

OUTPUT :-

$$\frac{y}{x+y} - \frac{xy}{(x+y)^2}$$

$$\frac{x}{x+y} - \frac{xy}{(x+y)^2}$$

Aim :- Second order partial derivative

```
1) var('x, y')  
f(x, y) = (x*y) / (x + y)  
fx = f.diff(x)  
show(fx(x, y))  
fy = f.diff(y)  
show(fy(x, y))  
fxx = f.diff(x, 2)  
show(fxx(x, y))
```


$f_{yy} = f.\text{diff}(y, 2)$
show($f_{yy}(x, y)$)

OUTPUT :-

$$\frac{y}{x+y} - \frac{xy}{(x+y)^2}$$
$$\frac{x}{x+y} - \frac{xy}{(x+y)^2}$$
$$- \frac{2y}{(x+y)^2} + \frac{2xy}{(x+y)^3}$$

First order partial derivative

$$f(x) = \frac{xy}{(x+y)}$$

Diff. w.r.t. 'x'

$$f'(x) = \frac{(x+y) \cdot y(1) - xy(1+0)}{(x+y)^2}$$

$$= \frac{(x+y)y}{(x+y)^2} - \frac{xy}{(x+y)^2}$$

$$= \frac{y}{(x+y)} - \frac{xy}{(x+y)^2}$$

$$f(y) = \frac{xy}{x+y}$$

Diff. w.r.t. 'y'

$$f'(y) = \frac{(x+y) \cdot x(1) - xy(0+1)}{(x+y)^2}$$

$$f'(y) = \frac{(x+y) \cdot x - xy}{(x+y)^2}$$

$$f'(y) = \frac{(x+y)(xy)}{(x+y)^2} - \frac{xy}{(x+y)^2}$$

$$f'(y) = \frac{x}{(x+y)} - \frac{xy}{(x+y)^2}$$

Second order partial derivative

$$f'(x) = \frac{y}{(x+y)} - \frac{xy}{(x+y)^2}$$

$$f''(x) = y \left(\frac{-1}{(x+y)^2} \right) - \left[\frac{(x+y)^2 y(1) - xy(2(x+y)(1+0))}{((x+y)^2)^2} \right]$$

$$= \frac{-y}{(x+y)^2} - \left[\frac{(x+y)^2 y - 2xy(x+y)}{(x+y)^4} \right]$$

$$= \frac{-y}{(x+y)^2} - \left[x+y \left(\frac{(x+y)y - 2xy}{(x+y)^4} \right) \right]$$

$$= \frac{-y}{(x+y)^2} - \left[\frac{(x+y)y - 2xy}{(x+y)^3} \right]$$

$$= \frac{-y}{(x+y)^2} - \left[\frac{(x+y)y + 2xy}{(x+y)^3} \right]$$

$$= \frac{-y}{(x+y)^2} - \frac{y}{(x+y)^2} + \frac{2xy}{(x+y)^3}$$

$$= \frac{-2y}{(x+y)^2} + \frac{2xy}{(x+y)^3}$$

$$f''(y) = \frac{x}{(x+y)} - \frac{xy}{(x+y)^2}$$

$$f''(y) = x \left(\frac{-1}{(x+y)^2} \right) - \left[\frac{(x-y)^2 \times (1) - xy(2(x+y)[0+1])}{((x+y)^2)^2} \right]$$

$$= \frac{-x}{(x+y)^2} - \left[\frac{(x+y)^2 x - 2xy(x+y)}{(x+y)^4} \right]$$

$$= \frac{-x}{(x+y)^2} - \left[\frac{(x+y) [(x+y)x - 2xy]}{(x+y)^4} \right]$$

$$= \frac{-x}{(x+y)^2} - \left[\frac{(x+y)x}{(x+y)^3} - \frac{2xy}{(x+y)^3} \right]$$

$$= \frac{-x}{(x+y)^2} - \frac{x}{(x+y)^2} + \frac{2xy}{(x+y)^3}$$

$$= \frac{-x - x}{(x+y)^2} + \frac{2xy}{(x+y)^3}$$

=

$$= \frac{-2x}{(x+y)^2} + \frac{2xy}{(x+y)^3}$$

Practical - 8

Aim:- Directional derivatives

$$1) D_{\mathbf{u}} f(x_0, y_0) = f_x(x_0, y_0)u_1 + f_y(x_0, y_0)u_2$$

var('x, y')

$$f(x, y) = 4 * x * y * \exp(-x^2 - y^2)$$

$$(a, b) = 1, 1$$

$$(u_1, u_2) = (1/\sqrt{2}, 1/\sqrt{2})$$

$$f.\text{diff}(x)(x=a, y=b) * u_1 + f.\text{diff}(y)(x=a, y=b) * u_2$$

OUTPUT:-

$$-4 * \sqrt{2} * e^{-2}$$

2) Gradient

var('x, y')

$$f(x, y) = x^2 * e^y$$

$$(a, b) = -2, 0$$

$$v = f.\text{gradient}() (x=a, y=b)$$

show(v)

OUTPUT:-

$$(-4, 4)$$

$$= \frac{1}{\sqrt{2}} ; u_2 = \frac{1}{\sqrt{2}} ; x_0 = 1 ; y_0 = 1$$

$$f(x, y) = 4xy e^{(-x^2 - y^2)}$$

$$\rightarrow f_x(x_0, y_0) = 4y [x e^{(-x^2 - y^2)} (-2x) + e^{(-x^2 - y^2)}] (1)$$

$$\begin{aligned}
 f_x(1,1) &= 4(1)[(1) \cdot e^{(-1)^2 - (1)^2} (-2) + e^{(-1)^2 - (1)^2}] \\
 &= 4[e^{-2}(-2) + e^{-2}] \\
 &= e^{-2} 4(-2+1) \\
 &= -4e^{-2} \quad \text{--- (i)}
 \end{aligned}$$

$$\begin{aligned}
 f_y(x_0, y_0) &= 4x[y e^{(-x^2 - y^2)} (-2y) + e^{(-x^2 - y^2)} (1)] \\
 f_y(1,1) &= 4(1)[(1) e^{(-1)^2 - (1)^2} (-2(1)) + e^{(-1)^2 - (1)^2}] \\
 &= 4[e^{-2}(-2) + e^{-2}] \\
 &= 4e^{-2}[-2+1] \\
 &= -4e^{-2} \quad \text{--- (ii)}
 \end{aligned}$$

By substituting in formula,

$$\begin{aligned}
 u f(x_0, y_0) &= f_x(x_0, y_0) x_1 + f_y(x_0, y_0) x_2 \\
 &= \frac{(-4e^{-2})}{\sqrt{2}} + \frac{(-4e^{-2})}{\sqrt{2}} \quad \text{--- (from (i) & (ii))} \\
 &= \frac{-4e^{-2} + (-4e^{-2})}{\sqrt{2}} \\
 &= \frac{-8e^{-2}}{\sqrt{2}} \\
 &= -4\sqrt{2} \times e^{-2}
 \end{aligned}$$

Practical - 9

Aim:- Tangent Planes and Normal Vectors for functions of two or three variables.

```
1) var('x, y, z')
f(x, y) = x^2 + 4*y^2 + z^2
(a, b, c) = (1, 2, 1)
fx = f.diff(x)(x=a, y=b, z=c)
fy = f.diff(y)(x=a, y=b, z=c)
fz = f.diff(z)(x=a, y=b, z=c)
T(x, y) = fx*(x-a) + fy*(y-b) + fz*(z-c)
show(T(x, y))
n = (fx, fy, fz)
show(n)
```

OUTPUT:-

$$2x + 16y + 2z - 36$$
$$(2, 16, 2)$$

$$x^2 + 4y^2 + z^2; (x, y, z) \equiv (1, 2, 1)$$

$$f_x(x^2 + 4y^2 + z^2) = 2x$$

$$f_y(x^2 + 4y^2 + z^2) = 8y$$

$$f_z(x^2 + 4y^2 + z^2) = 2z$$

$$\nabla f(x, y, z) = [f_x(x, y, z), f_y(x, y, z), f_z(x, y, z)]$$

$$\nabla f(1, 2, 1) = [2x, 8y, 2z]$$

$$= [2(1), 8(2), 2(1)]$$

$$= [2, 16, 2]$$

eqⁿ of tangent plane,

$$f_x(x, y, z)(x - x_0) + f_y(x, y, z)(y - y_0) + f_z(x, y, z)(z - z_0) = 0$$

$$2(x - 1) + 16(y - 2) + 2(z - 1) = 0$$

$$2x - 2 + 16y - 32 + 2z - 2 = 0$$

$$2x + 16y + 2z - 36 = 0$$